experiments/rupicola/StlcStrongDbParSubst.fst
@@ -1,0 +1,224 @@
+(*
+   Copyright 2014-2015
+     Simon Forest - Inria and ENS Paris
+     Catalin Hritcu - Inria
+     Nikhil Swamy - Microsoft Research
+
+   Licensed under the Apache License, Version 2.0 (the "License");
+   you may not use this file except in compliance with the License.
+   You may obtain a copy of the License at
+
+       http://www.apache.org/licenses/LICENSE-2.0
+
+   Unless required by applicable law or agreed to in writing, software
+   distributed under the License is distributed on an "AS IS" BASIS,
+   WITHOUT WARRANTIES OR CONDITIONS OF ANY KIND, either express or implied.
+   See the License for the specific language governing permissions and
+   limitations under the License.
+*)
+
+module StlcStrongDbParSubst
+
+open FStar.Constructive
+open FStar.Classical
+open FStar.FunctionalExtensionality
+open FStar.StrongExcludedMiddle
+
+(* Constructive-style progress and preservation proof for STLC with
+   strong reduction, using deBruijn indices and parallel substitution. *)
+
+type typ =
+  | TArr  : typ -> typ -> typ
+  | TUnit : typ
+
+type var = nat
+
+type exp =
+  | EVar  : var -> exp
+  | EApp  : exp -> exp -> exp
+  | ELam  : typ -> exp -> exp
+  | EUnit : exp
+
+(* Parallel substitution operation `subst` *)
+
+(* The termination argument uses a lexicographic ordering composed of:
+   0) a bit saying whether the expression is a variable or not;
+   1) an _undecidable_ well-founded order on substitutions that
+      equates all renamings, equates all non-renamings, and makes
+      renamings strictly smaller than non-renamings; we write down a
+      non-constructive function is_renaming mapping substitutions
+      (infinite objects) to 0 (renaming) or 1 (non-renaming)
+   2) the structure of the expression e *)
+
+type sub = var -> Tot exp
+
+type renaming (s:sub) = (forall (x:var). EVar? (s x))
+
+val is_renaming : s:sub -> GTot (n:int{  (renaming s  ==> n=0) /\
+                                       (~(renaming s) ==> n=1)})
+let is_renaming s = (if strong_excluded_middle (renaming s) then 0 else 1)
+
+
+val sub_inc : var -> Tot exp
+let sub_inc y = EVar (y+1)
+
+val renaming_sub_inc : unit -> Lemma (renaming (sub_inc))
+let renaming_sub_inc _ = ()
+
+let is_var (e:exp) : int = if EVar? e then 0 else 1
+
+val sub_elam: s:sub -> var -> Tot (e:exp{renaming s ==> EVar? e})
+                                (decreases %[1;is_renaming s; 0; EVar 0])
+val subst : s:sub -> e:exp -> Pure exp (requires True)
+     (ensures (fun e' -> (renaming s /\ EVar? e) ==> EVar? e'))
+     (decreases %[is_var e; is_renaming s; 1; e])
+let rec subst s e =
+  match e with
+  | EVar x -> s x
+  | ELam t e1 -> ELam t (subst (sub_elam s) e1)
+  | EApp e1 e2 -> EApp (subst s e1) (subst s e2)
+  | EUnit -> EUnit
+
+and sub_elam s y = if y=0 then EVar y
+                   else subst sub_inc (s (y-1))
+
+val sub_beta : exp -> Tot sub
+let sub_beta v = fun y -> if y = 0 then v      (* substitute *)
+                          else (EVar (y-1))    (* shift -1 *)
+
+(* Small-step operational semantics; strong / full-beta reduction is
+   non-deterministic, so necessarily as inductive relation *)
+
+type step : exp -> exp -> Type =
+  | SBeta : t:typ ->
+            e1:exp ->
+            e2:exp ->
+            step (EApp (ELam t e1) e2) (subst (sub_beta e2) e1)
+  | SApp1 : #e1:exp ->
+             e2:exp ->
+            #e1':exp ->
+            $hst:step e1 e1' ->
+                 step (EApp e1 e2) (EApp e1' e2)
+  | SApp2 :  e1:exp ->
+            #e2:exp ->
+            #e2':exp ->
+            $hst:step e2 e2' ->
+                 step (EApp e1 e2) (EApp e1 e2')
+
+(* Type system; as inductive relation (not strictly necessary for STLC) *)
+
+type env = var -> Tot (option typ)
+
+val empty : env
+let empty _ = None
+
+(* we only need extend at 0 *)
+val extend : typ -> env -> Tot env
+let extend t g y = if y = 0 then Some t
+                   else g (y-1)
+
+noeq type typing : env -> exp -> typ -> Type =
+  | TyVar : #g:env ->
+             x:var{Some? (g x)} ->
+             typing g (EVar x) (Some?.v (g x))
+  | TyLam : #g :env ->
+             t :typ ->
+            #e1:exp ->
+            #t':typ ->
+            $hbody:typing (extend t g) e1 t' ->
+                   typing g (ELam t e1) (TArr t t')
+  | TyApp : #g:env ->
+            #e1:exp ->
+            #e2:exp ->
+            #t11:typ ->
+            #t12:typ ->
+            $h1:typing g e1 (TArr t11 t12) ->
+            $h2:typing g e2 t11 ->
+                typing g (EApp e1 e2) t12
+  | TyUnit : #g:env ->
+             typing g EUnit TUnit
+
+(* Progress *)
+
+val is_value : exp -> Tot bool
+let is_value e = ELam? e || EUnit? e
+
+val progress : #e:exp -> #t:typ -> h:typing empty e t ->
+                         Pure (cexists (fun e' -> step e e'))
+                              (requires (~ (is_value e)))
+                              (ensures (fun _ -> True)) (decreases h)
+let rec progress #e #t h =
+  match h with
+  | TyApp #g #e1 #e2 #t11 #t12 h1 h2 ->
+     match e1 with
+     | ELam t e1' -> ExIntro (subst (sub_beta e2) e1') (SBeta t e1' e2)
+     | _          -> let ExIntro e1' h1' = progress h1 in
+                     ExIntro (EApp e1' e2) (SApp1 e2 h1')
+
+module T = FStar.Tactics.V2
+
+(* Substitution extensional - used by substitution lemma below *)
+val subst_extensional: s1:sub -> s2:sub{feq s1 s2} -> e:exp ->
+                       Lemma (requires True)
+                             (ensures (subst s1 e = subst s2 e))
+                             [SMTPat (subst s1 e); SMTPat (subst s2 e)]
+let rec subst_extensional s1 s2 e =
+  match e with
+  | EVar _ -> ()
+  | ELam t e1 ->
+    assert (subst s1 (ELam t e1) == ELam t (subst (sub_elam s1) e1))
+      by T.norm [zeta; iota; delta_only [`%subst]];
+    assert (subst s2 (ELam t e1) == ELam t (subst (sub_elam s2) e1))
+      by T.norm [zeta; iota; delta_only [`%subst]];
+    subst_extensional (sub_elam s1) (sub_elam s2) e1
+  | EApp e1 e2 -> subst_extensional s1 s2 e1; subst_extensional s1 s2 e2
+  | _ -> ()
+
+(* Typing of substitutions (very easy, actually) *)
+type subst_typing (s:sub) (g1:env) (g2:env) =
+  (x:var{Some? (g1 x)} -> Tot(typing g2 (s x) (Some?.v (g1 x))))
+
+(* Substitution preserves typing
+   Strongest possible statement; suggested by Steven Schäfer *)
+val substitution :
+      #g1:env -> #e:exp -> #t:typ -> s:sub -> #g2:env ->
+      h1:typing g1 e t ->
+      hs:subst_typing s g1 g2 ->
+      Tot (typing g2 (subst s e) t)
+      (decreases %[is_var e; is_renaming s; e])
+let rec substitution #g1 #e #t s #g2 h1 hs =
+  match h1 with
+  | TyVar x -> hs x
+  | TyApp hfun harg -> TyApp (substitution s hfun hs) (substitution s harg hs)
+  | TyLam tlam hbody ->
+     let hs'' : subst_typing (sub_inc) g2 (extend tlam g2) =
+       fun x -> TyVar (x+1) in
+     let hs' : subst_typing (sub_elam s) (extend tlam g1) (extend tlam g2) =
+       fun y -> if y = 0 then TyVar y
+             else let n:var = y - 1 in //Silly limitation of implicits and refinements
+                  substitution sub_inc (hs n) hs'' //NS: needed to instantiate the Some?.v 
+     in TyLam tlam (substitution (sub_elam s) hbody hs')
+  | TyUnit -> TyUnit
+
+(* Substitution for beta reduction
+   Now just a special case of substitution lemma *)
+val substitution_beta :
+      #e:exp -> #v:exp -> #t_x:typ -> #t:typ -> #g:env ->
+      h1:typing g v t_x ->
+      h2:typing (extend t_x g) e t ->
+      Tot (typing g (subst (sub_beta v) e) t) (decreases e)
+let rec substitution_beta #e #v #t_x #t #g h1 h2 =
+  let hs : subst_typing (sub_beta v) (extend t_x g) g =
+    fun y -> if y = 0 then h1 else TyVar (y-1) in
+  substitution (sub_beta v) h2 hs
+
+(* Type preservation *)
+val preservation : #e:exp -> #e':exp -> #g:env -> #t:typ ->
+       ht:(typing g e t) ->
+       hs:step e e' ->
+       Tot (typing g e' t) (decreases ht)
+let rec preservation #e #e' #g #t (TyApp h1 h2) hs =
+  match hs with
+  | SBeta tx e1' e2' -> substitution_beta h2 (TyLam?.hbody h1)
+  | SApp1 e2' hs1   -> TyApp (preservation h1 hs1) h2
+  | SApp2 e1' hs2   -> TyApp h1 (preservation h2 hs2)
